Законы логики

3

$$ A \wedge_{}^{}(B \wedge_{}^{}C)=(A \wedge_{}^{}B) \wedge_{}^{}C $$


4
закон ассоциативности 

$$ (A \vee B) \vee = A \vee (B \vee C) $$


5 Закон дистрибутивности

$$ (A \wedge B)\vee C = (A \vee C)\wedge(B\vee C) $$


6 Закон дистрибутивности

$$ (A \vee B) \wedge C = (A \wedge C) \vee (B \wedge C) $$

7


13

$$ A \vee (A \wedge B)=A $$

14

$$ A \wedge_{}^{}(A \vee_{}^{}B)=A $$

15 

$$ \overline{A \wedge B} = \overline{A} \vee \overline{B} $$


16 

$$ \overline{A \vee_{}^{} B} = \overline{A} \ \wedge_{}^{}\overline{B} $$


17


 18 
 
 $$A\to B =  {\overline{A}}\vee  B$$


19

$$A\leftrightarrow B = ({\overline{A}}\vee B) \wedge  ({\overline{B}}\vee A)$$

20 

$$ A \Delta B = \left( \neg A \wedge  B \right) \vee \left( A \wedge \neg B \right) $$




