Законы.

1.

$$ A \wedge  B = B \wedge  A $$

3

$$ A\wedge_{}^{}(B\wedge_{}^{}C)=(A\wedge_{}^{}B)\wedge_{}^{}C $$

4

$$ (A \vee_{}^{} B) \vee C = A \vee(B \vee C) $$

5

$$ (A\bigwedge_{}^{}B)\bigvee_{}^{}C=(A\bigvee_{}^{}C)\bigwedge_{}^{}(B\bigvee_{}^{}C) $$

6

$$ (A \vee B) \wedge C=(A \wedge C) \vee (B \wedge C) $$

13

$$ A \wedge (A \vee_{}^{} B) = A $$

14 

$$ A \wedge(A \vee B) = A $$

15

$$ \overline{A \wedge B} = \overline{A} \vee \overline{B} $$

16 

$$ \overline{(a \wedge b)} = \overline{a} \vee \overline{b} $$

17 

$$ \(\bar {\bar A}=A\) $$

18

$$ A \to  B = \overline{A} \vee B $$

19 

$$ A\leftrightarrow B=(\bar{A} {\vee } B)\wedge (\bar{B} \vee A) $$

20

$$ A \oplus B = (\bar{A} \wedge  B) \vee (A \wedge  \bar{B)} $$


![image](https://user-images.githubusercontent.com/114549805/198816908-993696d3-9e8d-4103-b659-11318f5e5f4d.png)
